fixed the problems about recursive type and type definitions. 1) take one pass to collect all mapping from named types to their definition. 2) take the second pass to substitute type names by their definitions.
git-svn-id: https://webdav.seas.upenn.edu/svn/sol/vol@2949 eef5ea85-cc2e-0410-bd84-0fae1f012da8

src/ssa/genericvalues.v
@@ -159,8 +159,43 @@ with typs2utyps_aux (m:list(id*typ)) (ts:list_typ) : option list_typ :=
      ret (Cons_list_typ ut0 uts0)
  end.
 
-Definition typ2utyp (nts:namedts) (t:typ) : option typ :=
+Definition typ2utyp' (nts:namedts) (t:typ) : option typ :=
 let m := gen_utyp_maps (List.rev nts) in
+typ2utyp_aux m t.
+
+Fixpoint subst_typ (i':id) (t' t:typ) : typ :=
+ match t with
+ | typ_int _ | typ_floatpoint _ | typ_void | typ_label | typ_metadata 
+ | typ_opaque => t
+ | typ_array s t0 => typ_array s (subst_typ i' t' t0)
+ | typ_function t0 ts0 => 
+     typ_function (subst_typ i' t' t0) (subst_typs i' t' ts0)
+ | typ_struct ts0 => typ_struct (subst_typs i' t' ts0)
+ | typ_pointer t0 => typ_pointer (subst_typ i' t' t0)
+ | typ_namedt i => if (eq_atom_dec i i') then t' else t
+ end
+with subst_typs (i':id) (t':typ) (ts:list_typ) : list_typ := 
+ match ts with
+ | Nil_list_typ => Nil_list_typ
+ | Cons_list_typ t0 ts0 =>
+     Cons_list_typ (subst_typ i' t' t0) (subst_typs i' t' ts0)
+ end.
+
+Fixpoint subst_typ_by_nts (nts:namedts) (t:typ) : typ :=
+match nts with
+| nil => t
+| (namedt_intro id' t')::nts' => subst_typ_by_nts nts' (subst_typ id' t' t)
+end.
+
+Fixpoint subst_nts_by_nts (nts0 nts:namedts) : list (id*typ) :=
+match nts with
+| nil => nil
+| (namedt_intro id' t')::nts' => 
+    (id',(subst_typ_by_nts nts0 t'))::subst_nts_by_nts nts0 nts'
+end.
+
+Definition typ2utyp (nts:namedts) (t:typ) : option typ :=
+let m := subst_nts_by_nts nts nts in
 typ2utyp_aux m t.
 
 Fixpoint mgetoffset_aux (TD:TargetData) (t:typ) (idxs:list Z) (accum:Z) 
